## Example 1: Combining Fractions

**Problem**

Simplify 
$$\frac{3}{x+1} - \frac{1}{2x+2} = 5$$.

**Solution**

$$
\begin{align*}
\frac{3}{x+1} - \frac{1}{2x+2} &= 5\\
\frac{3}{x+1} - \frac{1}{2(x+1)} &= 5\\
\frac{3(2)}{2(x+1)} - \frac{1}{2(x+1)} &= 5\\
\frac{6-1}{2(x+1)} &= 5\\
\frac{5}{2x+2} &= 5\\
5 &= 5(2x + 2)\\
5 &= 10x + 10\\
-10x &= 10 - 5\\
-10x &= 5\\
x &= -\frac{5}{10}\\
x &= -\frac{1}{2}
\end{align*}
$$

## Practice 1.1

**Problem**

Solve $$\frac{2x+7}{x-5} + \frac{5(x-2)}{5-x} = -13$$.

**Answer**

$$4\frac{4}{5}$$

## Practice 1.2

**Problem**

Solve $$\frac{1}{3x-2} - \frac{2x}{6-9x} = 3$$.

**Answer**

$$\frac{21}{25}$$

## Practice 1.3

**Problem**

$$
\frac{2x}{x+2} - \frac{3}{x^2 + 5x + 6} = 2.
$$

**Answer**

$$2\frac{1}{6}$$


## Example 2

**Problem**

Solve the equation

$$
\frac{7}{3x - 1} = \frac{8}{x + 5}
$$

**Solution**

$$
\begin{align*}
\frac{7}{3x-1} &= \frac{8}{x+5} \\
7(x+5) &= 8(3x-1) \\
7x+35 &= 24x-8 \\
7x-24x &= -8-35 \\
-17x &= -43 \\
x &= \frac{43}{17} \\
x &= 2\frac{9}{17}
\end{align*}
$$

## Example 3

**Problem**

Solve

$$
\frac{2}{x - 5} = \frac{8 - 3x}{x^2 - 25}
$$

**Solution**

$$
\begin{align*}
\frac{2}{x - 5} &= \frac{8 - 3x}{x^2 - 25} \\
\frac{2}{x - 5} &= \frac{8 - 3x}{(x - 5)(x + 5)} \\
2(x + 5) &= (8 - 3x)(x - 5) \\
2x + 10 &= 8 - 3x \\
2x + 3x &= 8 - 10 \\
5x &= -2 \\
x &= -\frac{2}{5}
\end{align*}
$$

## Example 4

**Problem**

Solve

$$
\frac{3}{x-4} - \frac{x-5}{(x-4)(2x+3)} = \frac{4}{2x+3}
$$

**Solution**

$$
\begin{align*}
\frac{3}{x-4} - \frac{x-5}{(x-4)(2x+3)} &= \frac{4}{2x+3} \\
\frac{3(2x+3)}{(x-4)(2x+3)} - \frac{x-5}{(x-4)(2x+3)} &= \frac{4}{2x+3} \\
\frac{3(2x+3) - (x-5)}{(x-4)(2x+3)} &= \frac{4}{2x+3} \\
\frac{(6x+9) - (x+5)}{(x-4)(2x+3)} &= \frac{4}{2x+3} \\
\frac{5x+14}{(x-4)(2x+3)} &= \frac{4}{2x+3} \\
5x+14 &= 4(x-4) \\
5x+14 &= 4x-16 \\
5x-4x &= -16-14 \\
x &= -30
\end{align*}
$$

## Example 5

**Problem**

Solve

$$
\frac{4x}{2x-3} - 2 = \frac{1}{2-3x}
$$

**Solution**

$$
\begin{align*}
\frac{4x}{2x-3} - 2 &= \frac{1}{2-3x} \\
\frac{4x}{2x-3} - \frac{4x-6}{2x-3} &= \frac{1}{2-3x} \\
\frac{6}{2x-3}  &= \frac{1}{2-3x} \\
6(2-3x) &= 2x-3 \\
12 - 18x &= 2x-3 \\
15 &= 20x \\
x &= \frac{3}{4}  \\
\end{align*}
$$





<!--stackedit_data:
eyJoaXN0b3J5IjpbLTE3MjUyMjA2OTJdfQ==
-->